books/centaur/aignet/litp.lisp
@@ -20,10 +20,10 @@
 ;                   Jared Davis <jared@centtech.com>
 
 (in-package "AIGNET")
-(local (include-book "centaur/bitops/ihsext-basics" :dir :system))
 (include-book "std/util/define" :dir :system)
 (include-book "std/basic/defs" :dir :system)
 (include-book "centaur/misc/arith-equivs" :dir :system)
+(local (include-book "centaur/bitops/ihsext-basics" :dir :system))
 (set-tau-auto-mode nil)
 
 
