books/centaur/bitops/extra-defs.lisp
@@ -19,12 +19,12 @@
 ; Original author: Jared Davis <jared@centtech.com>
 
 (in-package "ACL2")
-(local (include-book "ihsext-basics"))
-(local (include-book "arithmetic/top" :dir :system))
 (include-book "std/util/define" :dir :system)
 (include-book "std/basic/defs" :dir :system)
 (include-book "centaur/misc/arith-equivs" :dir :system)
 (include-book "ihs/logops-definitions" :dir :system)
+(local (include-book "ihsext-basics"))
+(local (include-book "arithmetic/top" :dir :system))
 (local (include-book "signed-byte-p"))
 
 (defsection bitops/extra-defs
