books/centaur/esim/esim-cut.lisp
@@ -25,13 +25,13 @@
 (in-package "ACL2")
 (include-book "esim-primitives")
 (include-book "esim-paths")
-(local (include-book "esim-sexpr-support-thms"))
 (include-book "std/util/define" :dir :system)
 (include-book "std/util/defaggregate" :dir :system)
 (include-book "std/util/defprojection" :dir :system)
 (include-book "std/util/defalist" :dir :system)
 (include-book "std/util/defmapappend" :dir :system)
 (include-book "centaur/vl/toe/toe-emodwire" :dir :system)
+(local (include-book "esim-sexpr-support-thms"))
 
 #||
 (include-book
