books/std/strings/html-encode.lisp
@@ -21,9 +21,9 @@
 (in-package "STR")
 (include-book "cat")
 (include-book "tools/bstar" :dir :system)
+(include-book "misc/definline" :dir :system)  ;; bozo
 (local (include-book "misc/assert" :dir :system))
 (local (include-book "arithmetic"))
-(include-book "misc/definline" :dir :system)  ;; bozo
 
 (defsection html-encoding
   :parents (std/strings)
