books/std/strings/istrprefixp.lisp
@@ -22,9 +22,9 @@
 (include-book "ieqv")
 (include-book "iprefixp")
 (include-book "std/basic/defs" :dir :system)
+(include-book "misc/definline" :dir :system)  ;; bozo
 (local (include-book "std/lists/nthcdr" :dir :system))
 (local (include-book "arithmetic"))
-(include-book "misc/definline" :dir :system)  ;; bozo
 
 (local (defthm iprefixp-lemma-1
          (implies (and (natp xn)
